Make FileId equality work on MockIds. MockIds use a list of pairs rather than ByteData. Move gunzip to a hypothesis of the definitions

FileIds.v
@@ -1,17 +1,24 @@
+Require Import Coq.Lists.List.
 Require Import Coq.ZArith.ZArith.
 
+Require Import Byte.
 Require Import ByteData.
+Require Import Util.
+
+Local Open Scope bool.
+Local Open Scope N.
 
 Inductive FileId: Type :=
   | Ext2Id: N -> FileId
   | TarId: FileId -> N -> FileId
-  | MockId: ByteData -> FileId
+  | MockId: list (N*Byte) -> FileId
 .
 
 Fixpoint eqb (lhs rhs: FileId) :=
   match (lhs, rhs) with
   | ((Ext2Id l), (Ext2Id r)) => N.eqb l r
   | ((TarId lfs l), (TarId rfs r)) => (andb (eqb lfs rfs) (N.eqb l r))
+  | ((MockId l), (MockId r)) => listN_Byte_eqb l r
   | _ => false
   end.
 
@@ -34,6 +41,8 @@ Proof.
       reflexivity.
     (* MockId *)
     destruct rhs0; 
-      [simpl; intros; inversion H | simpl; intros; inversion H | 
-       simpl; intros; inversion H].
+      [simpl; intros; inversion H | simpl; intros; inversion H |].
+      intros. unfold eqb in H.
+      apply listN_Byte_eqb_reflection in H.
+      rewrite H. reflexivity.
 Qed.
