HoneynetDefinitions.v
@@ -6,26 +6,30 @@ Require Import FileData.
 Require Import FileTypes.
 Require Import Tar.
 
-Open Local Scope bool.
+Variable gunzip: File->File.
 
-Definition borland_rootkit (disk: Disk) (gunzip: File->File) :=
+Local Open Scope bool.
+
+Definition borland_rootkit (disk: Disk) :=
   exists file: File,
     isOnDisk file disk
     /\ isDeleted file
     /\ isGzip file disk
     /\ Tar.looksLikeRootkit (gunzip file) disk.
 
-Definition borland_compute (disk: Disk) (gunzip: File->File)
-  (file: File) (filename1 filename2: string) :=
+Definition borland_compute (disk: Disk) (file gunzipped: File)
+  (filename1 filename2: string) :=
   (isOnDisk_compute file disk)
   && file.(deleted)
   && (isGzip_compute file disk)
-  && Tar.looksLikeRootkit_compute (gunzip file) disk filename1 filename2.
+  (*&& File.eqb gunzipped (gunzip file) *)
+  && Tar.looksLikeRootkit_compute gunzipped disk filename1 filename2.
 
-Lemma borland_reflection (disk: Disk) (gunzip: File->File)
-  (file: File) (filename1 filename2: string) :
-  borland_compute disk gunzip file filename1 filename2 = true
-    -> borland_rootkit disk gunzip.
+Lemma borland_reflection (disk: Disk) 
+  (file gunzipped: File) (filename1 filename2: string) :
+  borland_compute disk file gunzipped filename1 filename2 = true
+    -> (gunzip file) = gunzipped
+      -> borland_rootkit disk.
 Proof.
   intros. unfold borland_compute in H.
   apply Bool.andb_true_iff in H. destruct H.
@@ -36,5 +40,5 @@ Proof.
   split. apply isOnDisk_reflection. auto.
   split. unfold isDeleted. auto.
   split. apply isGzip_reflection. auto.
-  apply looksLikeRootkit_reflection in H0. auto.
+  rewrite H0. apply looksLikeRootkit_reflection in H1. auto.
 Qed.
